Proved election by teleportation

examples/Election.v
@@ -14,31 +14,38 @@ From TICL Require Import
   ICTree.Events.Writer.
 
 From Coq Require Import
-  Fin
   Lia
+  Fin
   Vector
-  List
   Classes.SetoidClass.
 
 From ExtLib Require Import
   Data.Monads.StateMonad.
 
+From Equations Require Import Equations.
+
 Set Implicit Arguments.
 
-Import TiclNotations ICTreeNotations.
+Import TiclNotations ICTreeNotations ICtree.
 Local Open Scope ictree_scope.
 Local Open Scope fin_vector_scope.
 Local Open Scope ticl_scope.
 
-Section Election.
-  Context (max: nat) (Hmax: max > 0).
-  Notation Id := { x: nat | x < max }.
+Module Type Cyclic.
+  Parameter (n: nat) (next: fin' n -> fin' n).
+End Cyclic.
 
+Module ElectionDefs(C: Cyclic).
+  Import C.
+  Notation Id := (fin' n). 
+  
   (*| Message passing in unidirectional ring |*)
   Variant msg :=
     | Candidate (u: Id)
     | Elected   (u: Id).
 
+  Notation Mails := (vec' n msg).
+  
   Variant netE: Type :=
     | Recv (from: Id)
     | Send (from: Id) (m: msg).
@@ -46,212 +53,258 @@ Section Election.
   Global Instance encode_netE: Encode netE :=
     fun e => match e with
           | Recv _ => msg
-          | Send _ _ => Id
+          | Send _ _ => unit
           end.
 
-  Definition send: Id -> msg -> ictree netE Id :=
-    fun i p => ICtree.trigger (Send i p).
+  Definition send: Id -> msg -> ictree netE unit :=
+    fun i p => trigger (Send i p).
 
   Definition recv: Id -> ictree netE msg :=
-    fun i => ICtree.trigger (Recv i).
+    fun i => trigger (Recv i).
 
-  Program Definition cycle(i: Id): Id :=
-    let n := proj1_sig i in
-    if PeanoNat.Nat.eq_dec (S n) max then
-      0
-    else
-      S n.
-  Next Obligation. lia. Defined.
-    
-  Notation Mails := (vec max msg).
-  Notation NetObs := (Id * msg).
-
-  Definition mget(mails: Mails)(id: Id): msg :=
-    mails $ of_nat_lt (proj2_sig id).
-
-  Definition mset(mails: Mails)(id: Id)(m: msg): Mails :=
-     mails @ (of_nat_lt (proj2_sig id)) := m.
-   
-  (* Local network instrumented semantics, write to [Mails] *)
-  Definition h_sysE'
-    : netE ~> stateT Mails (ictreeW NetObs) :=
+  (* Local network instrumented semantics, instrument [Send] *)
+  Definition h_netE
+    : netE ~> stateT Mails (ictreeW msg) :=
     fun e =>
       mkStateT
         (fun mails =>
-           match e return ictreeW (Id * msg) (encode e * Mails) with
+           match e return ictreeW msg (encode e * Mails) with
            | Send id msg =>
-               let next := cycle id in
-               Ret (next, mset mails next msg)
+               let next := next id in
+               Ret (tt, mails @ next := msg)
            | Recv id =>
-               let msg := mget mails id in
-               log (id, msg) ;;
+               let msg := mails $ id in
+               log msg ;;
                Ret (msg, mails)
            end).
+  
+  Lemma aur_recv: forall (x: Id) (ms: Mails) w,
+      not_done w ->
+      <[ {interp_state h_netE (recv x) ms}, w |=
+           AF (AX (done= {(ms $ x, ms)} {Obs (Log (ms $ x)) tt})) ]>.
+  Proof with eauto with ticl.
+    intros.
+    unfold recv, trigger.
+    rewrite interp_state_vis; cbn.
+    rewrite bind_bind.
+    apply aur_log.
+    - rewrite bind_ret_l, sb_guard, interp_state_ret.
+      cleft.
+      apply axr_ret...
+    - csplit...
+  Qed.
 
+  Lemma aur_send: forall (x: Id) (ms: Mails) (m: msg) w,
+    not_done w ->
+     <[ {interp_state h_netE (send x m) ms}, w |=
+         AF (AX (done= {(tt, ms @ (next x) := m)} w)) ]>.
+  Proof with eauto with ticl.
+    intros.
+    unfold send, trigger.
+    rewrite interp_state_vis; cbn.
+    rewrite bind_ret_l, sb_guard, interp_state_ret.
+    cleft.
+    apply axr_ret...
+  Qed.
+  
   (* Always terminates, conditional on receiving either:
      1. (Candidate candidate), where candidate = id -- I received my own [id] back
      2. (Elected leader) -- Someone else was elected [leader]
    *)
-  Definition elect(id: Id): ictree netE Id :=
+  Definition elect(id: Id): ictree netE unit :=
     m <- recv id ;;
     match m with
     | Candidate candidate =>
-        match Nat.eqb candidate id with (* candidate < id *)
+        match Fin_compare candidate id with (* candidate < id *)
         (* [left] neighbor proposed candidate, support her to [right]. *)
-        | Gt => send (Candidate candidate)
+        | Gt => send id (Candidate candidate)
         (* [left] neighbor proposed a candidate, do not support her. *)
         | Lt => Ret tt
         (* I am the leader, but only I know. Tell my [right] and return. *)
-        | Eq => send (Elected id)
+        | Eq => send id (Elected id)
         end
     | Elected leader =>
         (* I am a follower and know the [leader] *)
-        send (Elected leader)
+        send id (Elected leader)
     end.
 
   (* Uniring scheduler, picks initial [i] nondeterministically, then runs forever *)
-  Definition elect_sched'(cycle: fin' n -> fin' n): ictree sysE _ :=
-    i <- ICtree.branch n ;;
-    put i ;;
-    loop (
-        i <- get ;;
-        resumICtree (elect i) ;;
-        put (cycle i);;
-        continue
-      ).
+  Definition elect_sched: ictree netE void :=
+    i <- branch n ;;
+    iter (fun i =>
+            elect i ;;
+            Ret (inl (next i))
+      ) i.
 
-End Election.
+End ElectionDefs.
 
-From Equations Require Import Equations.
+Module Cyclic3 <: Cyclic.
+  Definition n:=2.
+  (* It is really hard to write [(a + 1) % n] with dependent fin for any n. *)
+  Equations next(i: fin' 2) : fin' 2 :=
+    next Fin.F1 := Fin.FS Fin.F1;
+    next (Fin.FS Fin.F1) := Fin.FS (Fin.FS Fin.F1);
+    next (Fin.FS (Fin.FS Fin.F1)) := Fin.F1.
+End Cyclic3.
+
 (* Run election for 3 workers *)
-Import Fin.
-Import VectorNotations.
+Import VectorNotations Vectors.
 Open Scope vector_scope.
 
-Equations cycle(i: fin' 2) : fin' 2 :=
-  cycle Fin.F1 := Fin.FS Fin.F1;
-  cycle (Fin.FS Fin.F1) := Fin.FS (Fin.FS Fin.F1);
-  cycle (Fin.FS (Fin.FS Fin.F1)) := Fin.F1.
+Module Election3.
+  Module E := ElectionDefs(Cyclic3).
+  Import E Cyclic3.
 
-Definition elect_sched := elect_sched' cycle.
-Definition h_sysE := h_sysE' cycle.
+  Notation id1 := Fin.F1.
+  Notation id2 := (Fin.FS (Fin.F1)).
+  Notation id3 := (Fin.FS (Fin.FS (Fin.F1))).
 
-(* Initial mailboxes are [F3, F1, F2] *)
-Definition mailboxes: vec' 2 (fin' 2) :=
-  Vector.cons _ (FS (FS F1)) _ (Vector.cons _ F1 _ (Vector.cons _ (FS F1) _ (Vector.nil _))).
+  Notation "{{ a , b , c }}" :=
+    (Vector.cons _ a _
+       (Vector.cons _ b _
+          (Vector.cons _ c _
+             (Vector.nil _)))).
 
-Import Vectors.
-Local Typeclasses Transparent equ.
-Local Typeclasses Transparent sbisim.
+  Ltac ddestruction3 x :=
+    dependent destruction x;
+    [| dependent destruction x;
+       [| dependent destruction x;
+          [| dependent destruction x]]].
 
-Ltac run_head :=
-  unfold iter, MonadIter_ictree;
-  rewrite interp_state_unfold_iter, interp_state_bind, bind_bind,
-    interp_state_vis, bind_bind;
-  cbn;
-  rewrite bind_ret_l, sb_guard, interp_state_ret, bind_ret_l, interp_state_bind, bind_bind,
-    interp_state_resumICtree, bind_vis, interp_state_vis, bind_bind;
-  cbn;
-  repeat setoid_rewrite bind_bind;
-  apply afl_log; eauto with ticl;
-  rewrite ?bind_ret_l, sb_guard, interp_state_bind, bind_bind,
-    interp_state_ret, bind_ret_l;
-  unfold resum_ret, ReSumRet_refl, ReSumRet_inr;
-  simp cycle; cbn.
+  Lemma next_neq: forall x,
+      next x <> x.
+  Proof.
+    intros.
+    ddestruction3 x; simp next; intros Hcontra; inv Hcontra.
+  Qed.
 
-Ltac run_body :=
-  rewrite interp_state_vis; cbn;
-  repeat setoid_rewrite bind_bind;
-  eapply afl_log; eauto with ticl;
-  rewrite ?bind_ret_l, sb_guard,
-        interp_state_ret, bind_ret_l, interp_state_bind, bind_bind,
-        interp_state_vis, bind_bind;
-  cbn;
-  rewrite bind_ret_l, sb_guard, interp_state_ret, bind_ret_l, interp_state_ret,
-    bind_ret_l, sb_guard;
-  simp cycle; cbn.
+  Lemma mget_mset_eq: forall (ms: Mails) (x: Id) m,
+      ((ms @ x := m) $ x) = m.
+  Proof.
+    intros.
+    repeat dependent destruction ms.
+    ddestruction3 x; simp next; cbn; reflexivity.
+  Qed.
+  
+  Lemma mget_mset_neq: forall (ms: Mails) (x: Id) m,
+      ((ms @ next x := m) $ x) = (ms $ x).
+  Proof.
+    intros.
+    repeat dependent destruction ms.
+    ddestruction3 x; simp next; cbn; reflexivity.
+  Qed.
 
-Ltac run_sched :=
-  rewrite interp_state_ret, bind_ret_l, interp_state_bind,
-    bind_bind, interp_state_vis, bind_bind;
-  cbn;
-  rewrite bind_ret_l, sb_guard,  interp_state_ret, bind_ret_l, interp_state_ret,
-    bind_ret_l, sb_guard;
-  simp cycle; cbn.
+  Definition ranking (id: Id) (mailboxes: Mails) :=
+    match id, mailboxes with
+    | id1, {{ Candidate id3, Candidate id1, Candidate id2 }} => 2
+    | id2, {{ Candidate id3, Candidate id3, Candidate id2 }} => 1
+    | id3, {{ Candidate id3, Candidate id3, Candidate id3 }} => 0
+    | id2, {{ Candidate id3, Candidate id1, Candidate id2 }} => 4
+    | id3, {{ Candidate id3, Candidate id1, Candidate id2 }} => 3
+    | _, _ => 10
+    end.
 
-Lemma election3_liveness:
-  <( {interp_state h_sysE elect_sched (F1, Vector.map Candidate mailboxes)}, Pure |=
-          AF visW {fun '(id, msg) => exists e, msg = Elected e /\ id = e /\ e = FS (FS F1)} )>.
-Proof with auto with ticl.
-  intros.
-  unfold elect_sched, elect_sched', ICtree.forever.
-  cbn.
-  rewrite interp_state_bind.
-  unfold ICtree.branch.
-  rewrite interp_state_br, bind_br.
-  apply aul_br; right; split.
-  - csplit...
-  - intros i.
-    unfold send, recv, put, get, ICtree.trigger.
-    rewrite sb_guard, interp_state_ret, bind_ret_l, interp_state_bind,
-      interp_state_vis, bind_bind.
-    cbn.
-    rewrite bind_ret_l, bind_guard, sb_guard, interp_state_ret, bind_ret_l,
-      interp_state_unfold_iter, interp_state_bind, bind_bind,
-      interp_state_vis, bind_bind.
-    cbn.
-    rewrite bind_ret_l, bind_guard, sb_guard, interp_state_ret, bind_ret_l,
-      interp_state_bind, bind_bind, interp_state_resumICtree.
-    (* Get into [elect] *)
+  (* Initial mailboxes are [F3, F1, F2] *)
+  Definition mailboxes: Mails :=
+    {{ Candidate id3, Candidate id1, Candidate id2 }}.
+
+  Lemma aur_elect: forall w (m' m: Mails) (i: Id) m',
+    not_done w ->
+    match m $ i with
+    | Candidate candidate =>
+        match Fin_compare candidate i with (* candidate < id *)
+        (* [left] neighbor proposed candidate, support her to [right]. *)
+        | Gt => m' = (m @ (next i) := (Candidate candidate))
+        (* [left] neighbor proposed a candidate, do not support her. *)
+        | Lt => m' = m
+        (* I am the leader, but only I know. Tell my [right] and return. *)
+        | Eq => m' = (m @ (next i) := (Elected i))
+        end
+    | Elected leader => m' = (m @ (next i) := (Elected leader))
+    end ->
+    <[ {interp_state h_netE (elect i) m}, {w} |= AF (AX (done= {(tt, m')} {Obs (Log (m $ i)) tt})) ]>.
+  Proof with eauto with ticl.
+    intros.
     unfold elect.
-    unfold send, recv, put, get, ICtree.trigger.
-    rewrite interp_state_bind, bind_bind, interp_state_vis, bind_bind.
-    cbn.
-    repeat setoid_rewrite bind_bind.
-    eapply afl_log...
-    rewrite ?bind_ret_l, sb_guard, interp_state_ret, bind_ret_l.
-    unfold resum_ret, ReSumRet_refl, ReSumRet_inl.
-    ddestruction i; [|ddestruction i; [|ddestruction i]]; simpl; simp cycle.
-    + (* Start with F1 *)
-      rewrite interp_state_vis, bind_bind.
-      cbn.
-      repeat setoid_rewrite bind_bind.
-      apply afl_log...
-      rewrite ?bind_ret_l, sb_guard.
-      (* sched *)
-      run_sched.
-      simp cycle; cbn.
-      (* F2 *)
-      run_head; run_body.
-      (* F3 *)
-      run_head; run_body.
-      (* Done *)
-      cleft; csplit.
-      eexists; intuition.
-    + (* sched *)
-      run_sched.
-      (* F3 *)
-      run_head; run_sched.
-      (* F1 *)
-      run_head; run_body.
-      (* F2 *)
-      run_head; run_body.
-      (* F3 *)
-      run_head; run_body.
-      (* Done *)
-      cleft; csplit.
-      eexists; intuition.
-    + (* F3 *)
-      run_sched.
-      (* F1 *)
-      run_head; run_body.
-      (* F2 *)
-      run_head; run_body.
-      (* F3 *)
-      run_head; run_body.
-      (* Done *)
-      cleft; csplit.
-      eexists; intuition.
-    + ddestruction i.
-Qed.
-Print Assumptions election3_liveness.
+    eapply aur_state_bind_r_eq.
+    - eapply aur_recv...
+    - destruct (m $ i) eqn:Hm.
+      + destruct (Fin_compare u i) eqn:Hcomp; subst.
+        * apply aur_send...
+        * cleft.
+          apply axr_state_ret...
+        * apply aur_send...
+      + subst.
+        apply aur_send...
+  Qed.
+
+  Ltac vroom :=
+    eapply aur_state_bind_r_eq;
+    [apply aur_elect; eauto with ticl; try exact mailboxes 
+    | cleft; apply axr_state_ret; eauto with ticl; eexists; intuition; simp next; eauto with ticl].
+
+  Local Typeclasses Transparent equ.
+  Local Typeclasses Transparent sbisim.
+  Lemma election3_liveness:
+    <( {interp_state h_netE elect_sched mailboxes}, Pure |= AF visW {fun msg => msg = Elected id3} )>.
+  Proof with eauto with ticl.
+    intros.
+    unfold elect_sched, mailboxes.
+    eapply aul_state_bind_r with (R:=fun _ σ' w' => σ' = mailboxes /\ w' = Pure).
+    - cright.
+    apply anr_state_br; split.
+      + csplit...
+      + intros.
+        apply aur_state_ret...
+    - intros * (-> & ->).
+      unfold mailboxes.
+      (* iter loop *)
+      eapply aul_state_iter_split_nat
+        with (Ri:=fun i ms w => (* Intermediate goal, full [Candidate id3] propagation *)
+                    w = Obs (Log (Candidate id3)) tt /\
+                      i = id3 /\
+                      ms = {{ Candidate id3, Candidate id3, Candidate id3 }})
+             (R:=fun (i: Id) (ms: Mails) (w: WorldW msg) =>
+                   match w with
+                   | Pure => i = x /\ ms = mailboxes
+                   | Obs (Log (Candidate p)) tt => 
+                       match (i, p) return _ = fin' 2 -> _ = fin' 2 -> Prop with
+                       | (id2, id3) => fun _ _ => ms = {{ Candidate id3, Candidate id3, Candidate id2 }}
+                       | (id3, id1) => fun _ _ => ms = {{ Candidate id3, Candidate id1, Candidate id2 }}
+                       | (id1, id2) => fun _ _ => ms = {{ Candidate id3, Candidate id1, Candidate id2 }}
+                       | _ => fun _ _ => False (* Only when w = Pure *)
+                       end eq_refl eq_refl
+                 | _ => False
+                 end)
+           (f:=fun id ms _ => ranking id ms)...
+    + (* Prove it gets to the intermediate state *)
+      intros; intuition; subst.
+      rename σ into m.
+      unfold mailboxes.
+      inv H.
+      * destruct H0 as (-> & ->).
+        unfold mailboxes.
+        ddestruction3 x; right.
+        -- (* x = 1 *) vroom.
+        -- (* x = 2 *) vroom.
+        -- (* x = 3 *) vroom.
+      * destruct e, v.
+        repeat ddestruction m.
+        destruct m0; try contradiction.
+        ddestruction3 i; ddestruction3 u; inv H0. 
+        -- (* i = 1, p = 3 *)
+          right. vroom.
+        -- (* i = 2, p = 3 *)
+          left. (* bingo! *)
+          vroom.
+        -- right. vroom.
+    + (* At checkpoint, now everything is deterministic *)
+      intros i w m _ (-> & ? & ->); subst.
+      eapply aul_state_iter_next_eq...
+      * vroom.
+      * do 2 (eapply aul_state_iter_next_eq; eauto with ticl; [vroom|simp next; cbn]).
+        cleft.
+        csplit...
+  Qed.
+  Print Assumptions election3_liveness.
+End Election3.
